Reorganizing for clarity.

model.v
@@ -6,10 +6,10 @@ Notation "'dec_type' T" := (forall x y : T, {x=y}+{x<>y}) (at level 70, no assoc
 Ltac split_refl eq_dec a := let H:= fresh in destruct (eq_dec a a) as [H|bad]; [clear H|contradict bad]; auto.
 Ltac split_refl2 eq_dec a a' := let H:= fresh in
                                 destruct (eq_dec a a') as [bad|H]; [contradict bad|clear H]; auto.
+Ltac inject_pair := match goal with [H: (?a, ?b) = (?c, ?d) |- _] => injection H; intros; subst end.
+Ltac inverts H := inversion H; subst.
 
-Definition name_eq_dec : dec_type Name.
-  decide equality.
-Defined.
+Definition name_eq_dec : dec_type Name. decide equality. Defined.
 Hint Immediate name_eq_dec.
 
 Generalizable All Variables.
@@ -20,57 +20,30 @@ Inductive Expr : Type :=
 | app : Expr -> Expr -> Expr
 | lam : Name -> Expr -> Expr.
 
-Definition expr_eq_dec : dec_type Expr.
-  decide equality.
-Defined.
+Definition expr_eq_dec : dec_type Expr. decide equality. Defined.
 Hint Immediate expr_eq_dec.
 
 Section Data.
 Variables Addr Time : Type.
 Variable addr_eq_dec : dec_type Addr.
 Variable time_eq_dec : dec_type Time.
-Hint Immediate addr_eq_dec time_eq_dec.
 
 Definition Env := list (Name * Addr).
-Definition env_eq_dec : dec_type Env.
-  apply list_eq_dec; decide equality.
-Defined.
-Hint Immediate env_eq_dec.
-
 Inductive storeable := s_closure : Name -> Expr -> Env -> storeable.
-Definition storeable_eq_dec : dec_type storeable. decide equality. Defined.
-Hint Immediate storeable_eq_dec.
-
 Definition AbsVal := set storeable.
-Definition absval_eq_dec : dec_type AbsVal. apply list_eq_dec; auto. Defined.
-Hint Immediate absval_eq_dec.
-
 Inductive val :=
   | closure : Name -> Expr -> Env -> val
   | adelay : Addr -> val
   | amany : AbsVal -> val.
-Definition val_eq_dec : dec_type val. decide equality. Defined.
-Hint Immediate val_eq_dec.
 
 Definition Store := list (Addr * AbsVal).
-Definition store_eq_dec : dec_type Store. apply list_eq_dec; decide equality. Defined.
-Hint Immediate store_eq_dec.
-
 Inductive Frame :=
   | ar : Expr -> Env -> Frame
   | fn : val -> Frame.
 
-Definition frame_eq_dec : dec_type Frame. decide equality. Defined.
-Hint Immediate frame_eq_dec.
-
 Definition Kont : Type := list Frame.
-
-Definition kont_eq_dec : dec_type Kont. apply list_eq_dec,frame_eq_dec. Defined.
-Hint Immediate kont_eq_dec.
-
 Inductive Shell (P : Type) :=
   shell : P -> Kont -> Time -> Shell P.
-
 Inductive CES_point :=
   | ev : Expr -> Env -> Store -> CES_point
   | co : val -> Store -> CES_point
@@ -78,19 +51,38 @@ Inductive CES_point :=
          val -> (* Argument *)
          Store -> CES_point.
 Definition CESK := Shell CES_point.
+
+Hint Immediate addr_eq_dec time_eq_dec.
+Definition env_eq_dec : dec_type Env. apply list_eq_dec; decide equality. Defined.
+Hint Immediate env_eq_dec.
+Definition storeable_eq_dec : dec_type storeable. decide equality. Defined.
+Hint Immediate storeable_eq_dec.
+Definition absval_eq_dec : dec_type AbsVal. apply list_eq_dec; auto. Defined.
+Hint Immediate absval_eq_dec.
+Definition val_eq_dec : dec_type val. decide equality. Defined.
+Hint Immediate val_eq_dec.
+Definition store_eq_dec : dec_type Store. apply list_eq_dec; decide equality. Defined.
+Hint Immediate store_eq_dec.
+Definition frame_eq_dec : dec_type Frame. decide equality. Defined.
+Hint Immediate frame_eq_dec.
+Definition kont_eq_dec : dec_type Kont. apply list_eq_dec,frame_eq_dec. Defined.
+Hint Immediate kont_eq_dec.
+Hint Constructors Shell.
+
 Definition store_of (p : CES_point) : Store :=
   match p with
       ev _ _ σ => σ
     | co _ σ => σ
     | ap _ _ _ _ σ => σ
   end.
+Hint Unfold Kont CESK store_of.
 
 Definition ces_point_eq_dec : dec_type CES_point. decide equality. Defined.
 Hint Immediate ces_point_eq_dec.
-
 Definition cesk_eq_dec : dec_type CESK. decide equality. Defined.
 Hint Immediate cesk_eq_dec.
 
+Section FiniteMaps.
 Inductive InDom {A B} : list (A * B) -> A -> Prop :=
   | dom_fst : `{InDom ((a,b)::rst) a}
   | dom_rst : `{InDom l a -> InDom ((a',b')::l) a}.
@@ -103,15 +95,9 @@ Inductive Unmapped {A B} : list (A * B) -> A -> Prop :=
   | unil : forall a, Unmapped nil a
   | ucons : forall a a' b l, Unmapped l a' -> a <> a' -> Unmapped ((a,b)::l) a'.
 
-Inductive Functional {A B} : list (A * B) -> Prop :=
-  | empty_fn : Functional nil
-  | extend_fn : `{Functional l -> Unmapped l a -> Functional ((a,b)::l)}.
-
 Lemma MapsTo_In : forall A B (l : list (A * B)) a b (H: MapsTo l a b), In (a,b) l.
 Proof.
-  induction l as [|(a,b) l' IH];
-  intros a' b' H; inversion H; (* finishes base case *)
-  subst; [constructor|right; apply IH]; auto.
+  induction l; intros ? ? H; inversion H; crush.
 Qed.
 
 Theorem InDom_is_mapped : forall A B (eq_dec : dec_type A) (l : list (A * B)) a, InDom l a <-> exists b, MapsTo l a b.
@@ -126,8 +112,6 @@ Proof.
     |rewrite IH in H'; destruct H' as [b H'']; exists b; constructor]
    |destruct H as [b H'']; inversion H''; subst; [contradict Hneq|constructor; rewrite IH; exists b]]; auto.
 Qed.
-
-Ltac inject_pair := match goal with [H: (?a, ?b) = (?c, ?d) |- _] => injection H; intros; subst end.
 
 Theorem InDom_In : forall A B (eq_dec : dec_type A) (l : list (A * B)) a, InDom l a <-> exists b, In (a,b) l.
 Proof.
@@ -159,26 +143,13 @@ Qed.
 
 Lemma in_not_unmapped : forall A B (l : list (A * B)) a b (H:In (a,b) l), ~ Unmapped l a.
 Proof.
-  induction l as [|(a,b) l' IH]; intros a0 b0 H bad; inversion H; subst.
+  induction l as [|(a,b) l' IH]; intros a0 b0 H bad; inverts H.
   inject_pair;
     inversion bad; auto.
   inversion bad as [|? ? ? ? bad']; apply IH with (b:= b0) in bad'; auto.
 Qed.
-
-
-Lemma in_functional_mapsto : forall A B (eq_dec : dec_type A) (l : list (A * B)) (F : Functional l)
-                                    a b (H : In (a,b) l), MapsTo l a b.
-Proof.
-  induction l as [|(a,b) l' IH];
-  intros F a' b' H; inversion H;[ (* finishes base case *)
-    inject_pair; subst; constructor; auto
-  |inversion F as [|? ? ? Hfun Hunmapped]; subst;
-   destruct (eq_dec a a'); [subst; contradict Hunmapped; apply in_not_unmapped with (b:=b')
-                           |constructor]]; auto.
-Qed.
-
-Remark functional_exchange : forall A B (l : list (A * B)) a b (F: Functional ((a,b)::l)) b', Functional ((a,b')::l).
-Proof. intros; inversion F; constructor; auto. Qed.
+End FiniteMaps.
+Hint Constructors InDom MapsTo Unmapped.
 
 Definition in_aval := @In storeable.
 
@@ -214,7 +185,7 @@ Proof.
   intros a' b'; split; intro H; simpl in *;
   destruct (eq_dec a' a) as [Hleft|Hright];
   solve
-   [inversion H;
+   [inversion H; 
    try solve [contradict Hleft; auto
              |contradict Hright; auto
              |apply IH; auto
@@ -316,18 +287,8 @@ Proof.
   induction l as [|(a,b) l_ IH]; intros a0 a' l' c H ?;
   simpl; repeat constructor; auto.
   simpl; destruct (eq_dec a' a) as [Heq|Hneq];
-  [subst; inversion H; constructor
+  [subst; inversion H
   |constructor;inversion H;[apply IH|]];auto.
-Qed.
-
-Lemma functional_join : `{Functional l -> Functional (list_join eq_dec combine base l' a c l)}.
-Proof.
-  induction l as [|(a,b) l_ IH]; simpl;
-  [intros; repeat constructor
-  |intros l' a' c F].
-  destruct (eq_dec a' a) as [Heq|Hneq];
-  [subst; apply functional_exchange with (b := b)
-  |constructor; inversion F; [apply IH|apply unmapped_join]]; auto.
 Qed.
 
 Lemma in_list_join2 :
@@ -341,7 +302,7 @@ Proof.
   [(* base case *) inversion Hpairin
   |destruct a0; destruct (eq_dec a a0) as [Heq | Hneq]; subst;
    [(* Heq *)
-     subst; inversion Hpairin; subst;
+     subst; inverts Hpairin;
     [exists (combine l' bs c); split; [left|apply Hextensive']; auto
            |exists bs; split; [right|]; auto]
    |(* Hneq *)
@@ -350,10 +311,10 @@ Proof.
     [exists bs; split; [constructor|]; auto
     |match goal with [Hbad : ?a <> ?a |- _] => contradict Hbad; auto end
     |exists bs; constructor; [constructor|]; auto
-    |assert (IHneed : in_list_list l a' c') by (exists bs; repeat constructor; auto);
+    |assert (IHneed : in_list_list l a' c') by (exists bs; auto);
      set (IHl_ := IHl IHneed);
      inversion IHl_ as [x Hwit]; destruct Hwit as [Hmap Hin];
-     exists x; repeat constructor; auto]]].
+     exists x; auto]]].
 Qed.
 
 Lemma non_join_untouched : forall l l' a a' c b
@@ -362,7 +323,7 @@ Lemma non_join_untouched : forall l l' a a' c b
                              MapsTo l a' b.
 Proof.
   induction l as [|(a_,b_) l_ IH]; intros;
-  [inversion H; subst; [contradict Hneq|]; auto
+  [inverts H; [contradict Hneq|]; auto
   |
   simpl in H; inversion H as [? ? rst H'|? a'' ? ? ? Hneq'' map' Hinj]; subst;
   destruct (eq_dec a a_) as [Heq_|Hneq_];
@@ -378,63 +339,6 @@ Proof.
   |subst; constructor; auto
   |constructor; [auto | apply IH with (l' := l') (a := a) (c := c); auto]]].
 Qed.
-
-(*
-  
-Lemma unmapped_join2 : forall l a a' b c l'
-                             (Hcontain : (forall a c, in_list_list l a c -> in_list_list l' a c)
-                                          \/ (b = (base l' c))),
-                        Unmapped l a' ->
-                        MapsTo (list_join eq_dec combine base l' a c l) a' b ->
-                        (b = (base l' c)) /\ a = a'.
-Proof.
-  induction l as [|(a_,b_) l_ IH];
-  simpl; intros a a' b c l' Hcontain Hunmap Hmap;
-  [inversion Hmap as [|? ? ? ? ? ? Hbad]; subst; split; solve [auto|reflexivity|inversion Hbad]
-  |].
-  destruct (eq_dec a a_) as [Heq | Hneq];
-    [inversion Hunmap as [|? ? ? ? Hunmap' Hneq]; subst;
-     inversion Hmap as [|? ? ? ? ? ? Hbad]; split; try solve [reflexivity|
-                                             rewrite unmapped_not_mapped in Hunmap';
-                                             [apply Hunmap' in Hbad; contradiction
-                                             |auto]]
-    |].
-  inversion Hmap as [|? ? ? ? ? ? Hbad]; subst; contradict Hneq; auto.
-  apply IH with (b := b) (c := c) (l' := l').
-  inversion Hcontain as [L|R].
-  specialize L with a_ b_
-  intros a_' c_' Hin; inversion Hin as [bs_ [Hmap_ Hsetin_]];
-  apply Hcontain; destruct (eq_dec a_' a_) as [Heq_|Hneq_];
-  [subst
-    |exists bs_; repeat constructor]; auto.
-  unfold in_list_list.
-  Focus 2.
-  
-    [intros a_' c_' Hin
-    |inversion Hunmap
-    |]; auto.
-
-; 
-  inversion Hmap; [(* a_' = a_ *)
-                   rewrite unmapped_not_mapped in Hunmap; [
-                    (* rewritten *)
-                    subst; match goal with [bad : ?a <> ?a |- _] => contradict bad; auto end
-                    |(* satisfy hyp *)assumption]
-                   |subst]. 
-  Check unmapped_not_mapped.
-                       
-   [specialize Hunmap with b; contradict Hunmap; constructor
-   |assumption
-   |
-   |assumption].
-  .
-  ; constructor; auto | auto].
-    
-
- subst; repeat constructor|]
-  constructor.
-Qed.
-Admitted.*)
 
 End ListJoin_facts.
 Section ListJoin_morefacts.
@@ -464,23 +368,23 @@ Proof.
 
   destruct (set_add_elim ceq_dec _ _ _ in_) as [Hceq|Hinrest];
        [intuition
-       |subst; right; exists cs; repeat constructor; auto].
+       |subst; right; exists cs; auto].
 
-  right; exists cs_; repeat constructor; auto.
+  right; exists cs_; auto.
 
   (* Neq case with inversion *)
-  right; exists cs_; repeat constructor; auto.
+  right; exists cs_; auto.
 
   destruct (eq_dec aa aa') as [Heq_|Hneq_].
   (* eq *)
   destruct IH with (l' := ll') (a := aa) (a' := aa') (c := cc) (c' := cc') as [S|S];
-    [exists cs_; constructor; auto
+    [exists cs_; auto
     |left; exact S
-    |inversion S as [ccs Hwit]; destruct Hwit as [mmap min]; right; exists ccs; split;[constructor|];auto].
+    |inversion S as [ccs Hwit]; destruct Hwit as [mmap min]; right; exists ccs; auto].
   (* neq *)
-  right.
+  right;
   apply non_join_untouched with (eq_dec := eq_dec) (combine := joiner) (base := singler) in too;
-    [exists cs_; repeat constructor|]; auto.
+    [exists cs_|]; auto.
 Qed.
     
 End ListJoin_morefacts.
@@ -536,6 +440,7 @@ Qed.
 Inductive KontTail : Kont -> Kont -> Prop :=
 | same_tail : `{KontTail κ κ}
 | push_tail : `{KontTail κ κ' -> KontTail κ (φ :: κ')}.
+Hint Constructors KontTail.
 
 Fixpoint kont_tailp (κ κ' : Kont) : bool :=
   match (kont_eq_dec κ κ') with
@@ -550,20 +455,20 @@ Lemma kont_tailp_correct1 : forall κ κ',
                              kont_tailp κ κ' = true -> KontTail κ κ'.
 Proof.
   induction κ'; simpl;
-  [destruct (kont_eq_dec κ nil); intro H; subst; try solve [constructor
+  [destruct (kont_eq_dec κ nil); intro H; subst; try solve [auto
                                                            |inversion H; contradiction]
-  |destruct (kont_eq_dec κ (a :: κ')) as [Heq|Hneq]; intro H; subst; try solve [constructor];
-   apply IHκ' in H; constructor]; auto.
+  |destruct (kont_eq_dec κ (a :: κ')) as [Heq|Hneq]; intro H; subst; auto;
+   apply IHκ' in H]; auto.
 Qed.
 
 Lemma kont_tailp_correct2 : forall κ κ',
                               KontTail κ κ' -> kont_tailp κ κ' = true.
 Proof.
   induction κ'; simpl;
-  [destruct (kont_eq_dec κ nil); intro H; subst; try solve [constructor
-                                                                  |inversion H; contradiction]
+  [destruct (kont_eq_dec κ nil); intro H; subst; try solve [auto
+                                                           |inversion H; contradiction]
   |destruct (kont_eq_dec κ (a :: κ')) as [Heq|Hneq]; intro H; subst; try solve [constructor];
-   apply IHκ'; inversion H; subst; [contradict Hneq|]; auto].
+   apply IHκ'; inverts H; [contradict Hneq|]; auto].
 Qed.
 
 Lemma kont_tail_nil : `{KontTail nil κ}.
@@ -571,7 +476,7 @@ Proof. induction κ as [|φ κ_ IH]; constructor; auto. Qed.
 
 Lemma kont_tail_cons : forall φ κ κ' (H : KontTail (φ::κ) κ'), KontTail κ κ'.
 Proof.
-  induction κ' as [|φ_ κ_ IH]; intros; inversion H; subst.
+  induction κ' as [|φ_ κ_ IH]; intros; inverts H.
   apply push_tail; constructor.
   apply push_tail,IH; auto.
 Qed.  
@@ -614,54 +519,40 @@ Inductive Trace {State} (s0 : State) (R : State -> State -> Prop) : list State -
                   R ς ς' ->
                   Trace s0 R (ς' :: (ς :: π))}.
 
-Definition CESK_trace (e : Expr) := Trace (shell (ev e nil nil) nil time0) red_cesk.
+Definition CESK_trace (e : Expr) := Trace (inject_cesk e) red_cesk.
 Section NonStandardData.
-Inductive Context :=
-  context : Expr -> Env -> Store -> Time -> Context.
-
-Definition context_eq_dec : dec_type Context.
-  decide equality; try solve [apply expr_eq_dec | apply env_eq_dec | apply store_eq_dec].
-Defined.
-
-Inductive Result :=
-  res: val -> Store -> Time -> Result.
+Inductive Context := context : Expr -> Env -> Store -> Time -> Context.
+Inductive Result := res: val -> Store -> Time -> Result.
 Definition Results := set Result.
-
-Definition result_eq_dec : dec_type Result.
-  decide equality; try solve [apply val_eq_dec | apply store_eq_dec].
-Defined.
 
 Inductive TrunKont :=
 | mt : TrunKont
 | kpush : Frame -> TrunKont -> TrunKont
 | rt : Context -> TrunKont.
 
-Definition trunkont_eq_dec : dec_type TrunKont.
-  decide equality; try solve [apply frame_eq_dec | apply context_eq_dec].
-Defined.
-
 Definition TrunKonts := set TrunKont.
 Definition Memo := list (Context * Results).
 Definition KTable := list (Context * TrunKonts).
 
+Definition context_eq_dec : dec_type Context. decide equality. Defined.
+Hint Immediate context_eq_dec.
+Definition result_eq_dec : dec_type Result. decide equality. Defined.
+Hint Immediate result_eq_dec.
+Definition trunkont_eq_dec : dec_type TrunKont. decide equality. Defined.
+Hint Immediate trunkont_eq_dec.
+
 Inductive TrunKontTail : TrunKont -> TrunKont -> Prop :=
 | same_ttail : `{TrunKontTail κ κ}
 | push_ttail : `{TrunKontTail κ κ' -> TrunKontTail κ (kpush φ κ')}.
-
+Hint Constructors TrunKontTail.
 Lemma trunkont_tail_kpush : forall tκ φ tκ', TrunKontTail (kpush φ tκ) tκ' -> TrunKontTail tκ tκ'.
 Proof.
-  induction tκ'; intro H; inversion H; subst; constructor; [constructor|apply IHtκ'; auto].
+  induction tκ'; intro H; inverts H; constructor; [|apply IHtκ']; auto.
 Qed.
 
-Definition memo_eq_dec : dec_type Memo.
-  decide equality;
-  decide equality; try solve [apply context_eq_dec | apply list_eq_dec, result_eq_dec].
-Defined.
-
-Definition ktable_eq_dec : dec_type KTable.
-  decide equality;
-  decide equality; try solve [apply context_eq_dec | apply list_eq_dec, trunkont_eq_dec].
-Defined.
+Definition memo_eq_dec : dec_type Memo. do 3 (decide equality). Defined.
+Definition ktable_eq_dec : dec_type KTable. do 3 (decide equality). Defined.
+Hint Immediate memo_eq_dec ktable_eq_dec.
 
 Definition trunckonts_join (κs κs' : TrunKonts) := set_union trunkont_eq_dec κs κs'.
 Definition lookup_M := lookup_map context_eq_dec (B := Results).
@@ -694,14 +585,24 @@ Fixpoint map_join {A B} (join1 : list (A * B) -> A -> B -> list (A * B)) (l l' :
       nil => l'
     | (a,b)::l'' => join1 (map_join join1 l'' l') a b
   end.
-Definition Ξs_join := map_join (fun Ξ ctx κs => list_join context_eq_dec
-                                                          (fun _ κs' κs => set_union trunkont_eq_dec κs' κs)
-                                                          (fun _ κs => κs)
-                                                          Ξ ctx κs Ξ).
-Definition Ms_join := map_join (fun M ctx rs => list_join context_eq_dec
-                                                          (fun _ rs' rs => set_union result_eq_dec rs' rs)
-                                                          (fun _ rs => rs)
-                                                          M ctx rs M).
+Definition mjoiner {A B} (Aeq_dec : dec_type A) (Beq_dec : dec_type B) (l : list (A * set B)) a bs :=
+  list_join Aeq_dec
+            (fun _ bs' bs => set_union Beq_dec bs' bs)
+            (fun _ bs => bs)
+            l a bs l.
+Definition Ξs_join := map_join (mjoiner context_eq_dec trunkont_eq_dec).
+Definition Ms_join := map_join (mjoiner context_eq_dec result_eq_dec).
+Lemma map_join_ordering1 : forall A B (Aeq_dec : dec_type A) (Beq_dec : dec_type B)
+                                 (l l' : list (A * set B)),
+                            MappingLE l (map_join (mjoiner Aeq_dec Beq_dec) l l').
+Proof.
+Admitted.
+
+Lemma map_join_ordering2 : forall A B (Aeq_dec : dec_type A) (Beq_dec : dec_type B)
+                                 (l l' : list (A * set B)),
+                            MappingLE l (map_join (mjoiner Aeq_dec Beq_dec) l' l).
+Proof.
+Admitted.
 
 Definition in_ctxs (Ξ : KTable) (ctx : Context) (κ : TrunKont) : Prop :=
   in_list_list Ξ ctx κ.
@@ -715,20 +616,17 @@ Inductive WShell (P : Type) :=
   wshell : P -> TrunKont -> Time -> WShell P.
 
 Definition WCESKMΞ := WShell CES_point.
-
-Definition wceskmξ_eq_dec : dec_type WCESKMΞ.
-  decide equality; try solve [apply ces_point_eq_dec | apply trunkont_eq_dec | apply time_eq_dec].
-Defined.
 Inductive CESKMΞ :=
   | widemk : WCESKMΞ -> Memo -> KTable -> CESKMΞ.
 
-Definition ceskmξ_eq_dec : dec_type CESKMΞ.
-  decide equality; try solve [apply wceskmξ_eq_dec | apply memo_eq_dec | apply ktable_eq_dec].
-Defined.
-
+Definition wceskmξ_eq_dec : dec_type WCESKMΞ. decide equality. Defined.
+Hint Immediate wceskmξ_eq_dec.
+Definition ceskmξ_eq_dec : dec_type CESKMΞ. decide equality. Defined.
+Hint Immediate ceskmξ_eq_dec.
 Section NonStandardSemantics.
 
-Definition inject_ceskmk (e : Expr) : CESKMΞ := widemk (wshell (ev e nil nil) mt time0) nil nil.
+Definition inject_wceskmk (e : Expr) : WCESKMΞ := (wshell (ev e nil nil) mt time0).
+Definition inject_ceskmk (e : Expr) : CESKMΞ := widemk (inject_wceskmk e) nil nil.
 Inductive red_ceskmk : CESKMΞ -> CESKMΞ -> Prop :=
   evmk_var : forall x ρ σ a tκ t M Ξ,
                let p := (ev (var x) ρ σ) in
@@ -781,14 +679,12 @@ Inductive red_ceskmk : CESKMΞ -> CESKMΞ -> Prop :=
 Inductive Dom_in_Dom {A B C} : list (A * B) -> list (A * C) -> Prop :=
   | no_dom : `{Dom_in_Dom nil l}
   | cons_dom : `{InDom l' a -> Dom_in_Dom l l' -> Dom_in_Dom ((a,b)::l) l'}.
-
+Hint Constructors Dom_in_Dom.
 Lemma Dom_InDom : forall A (eq_dec : dec_type A) B C (l : list (A * B)) (l' : list (A * C)) (Hdom : Dom_in_Dom l l')
                          a
                          (Hindom : InDom l a), InDom l' a.
 Proof.
-induction l; intros; [inversion Hindom|].
-inversion Hdom; subst.
-destruct (eq_dec a1 a0) as [Heq|Hneq]; [subst; auto|inversion Hindom; [subst; contradict Hneq|apply IHl]; auto].
+induction l; intros; [inversion Hindom|inverts Hdom;destruct (eq_dec a1 a0) as [Heq|Hneq]; [subst; auto|inversion Hindom; [subst; contradict Hneq|apply IHl]; auto]].
 Qed.
 
 Lemma In_join : forall A B C (eq_dec: dec_type A) (l l' : list (A * B))
@@ -798,7 +694,7 @@ Lemma In_join : forall A B C (eq_dec: dec_type A) (l l' : list (A * B))
                   (exists b'', In (a,b'') (list_join eq_dec f g l' a' b' l)).
 Proof.
   intros A B C eq_dec l l' f g a a' b b' Hcontain Hin; induction l as [|(a0,b0) l_ IH];
-  inversion Hin; subst;
+  inverts Hin;
   assert (IHneed : forall a b, In (a,b) l_ -> In (a,b) l') by
       (intros; apply Hcontain; right; auto);
   pose (rec := IH IHneed);
@@ -913,28 +809,20 @@ Inductive System :=
   system : set WCESKMΞ -> set WCESKMΞ -> Memo -> KTable -> System.
 
 
+Fixpoint smusher (S : set WCESKMΞ) (ss : set CESKMΞ) (nexts : set WCESKMΞ) (M : Memo) (Ξ : KTable) :=
+  match ss with
+      nil => wide_step (filter (fun s => if In_dec wceskmξ_eq_dec s S then false else true) nexts) M Ξ
+    | (widemk s M' Ξ')::ss' => smusher S ss' (set_add wceskmξ_eq_dec s nexts)
+                                     (Ms_join M' M)
+                                     (Ξs_join Ξ' Ξ)
+  end.
+
 Definition smush_steps (s : WCESKMΞ) (M: Memo) (Ξ: KTable) (S : set WCESKMΞ) : Wide_step :=
-  (fix smush (ss : set CESKMΞ) (nexts : set WCESKMΞ) (M : Memo) (Ξ : KTable) :=
-     match ss with
-         nil => wide_step (filter (fun s => if In_dec wceskmξ_eq_dec s S then false else true) nexts) M Ξ
-       | (widemk s M' Ξ')::ss' => smush ss' (set_add wceskmξ_eq_dec s nexts)
-                                        (Ms_join M' M)
-                                        (Ξs_join Ξ' Ξ)
-     end)
-    (step_all (widemk s M Ξ)) nil nil nil.
+  smusher S (step_all (widemk s M Ξ)) nil nil nil.
 
-Theorem finite_steps : forall s, exists ss : set CESKMΞ, forall s',
-                          (red_ceskmk s s' -> In s' ss) *
-                          (In s' ss -> red_ceskmk s s').
+Theorem finite_steps : forall s, forall s', (red_ceskmk s s' <-> In s' (step_all s)).
 Proof.
-  intro s; exists (step_all s); intro s'; split; [intro Hred|intro Hin].
-  inversion_clear Hred; simpl; try solve [left; auto|
-rewrite lookup_mapsto with (eq_dec := name_eq_dec) in H;
-unfold lookup_ρ; rewrite H; constructor; auto].
-inversion H.
 Admitted.
-
-Check smush_steps.
 
 Inductive Wide_CESKMΞ : System -> System -> Prop :=
   | big_step : forall s M Ξ Seen F ss M' Ξ',
@@ -945,7 +833,9 @@ Inductive Wide_CESKMΞ : System -> System -> Prop :=
                                   (set_union wceskmξ_eq_dec F ss)
                                   M' Ξ').
 
-Definition WCESKMΞ_trace (e : Expr) := Trace (system ((wshell (ev e nil nil) mt time0)::nil) ((wshell (ev e nil nil) mt time0)::nil) nil nil) Wide_CESKMΞ.
+Definition inject_wide_ceskmk (e : Expr) := (system [(inject_wceskmk e)] [(inject_wceskmk e)] nil nil).
+Definition WCESKMΞ_trace (e : Expr) :=
+  Trace (system [(inject_wceskmk e)] [(inject_wceskmk e)] nil nil) Wide_CESKMΞ.
 
 Inductive StackUnroll (Ξ : KTable) : Kont -> TrunKont -> Prop :=
   unroll_mt : `{StackUnroll Ξ nil mt}
@@ -1033,6 +923,7 @@ Proof with auto.
   apply unroll_inv with (κ := κ'); auto.
 Qed.  
 
+Section StackIrrelevance.
 Inductive hastail (κ : Kont) : list CESK -> Prop :=
   Nil_tail : hastail κ nil
 | Cons_tail : forall π p κ' t, hastail κ π -> KontTail κ κ' ->
@@ -1068,7 +959,7 @@ Fixpoint replacetail_kont (κ κ' κ'' : Kont) : option Kont :=
 Definition replacetail_kont_good : forall κ κ' κ'' (Htail : KontTail κ' κ),
                                      exists κ''', replacetail_kont κ κ' κ'' = Some κ'''.
 induction κ as [|φ κ_ IH]; intros;
-[exists κ''; inversion Htail; subst; simpl; reflexivity
+[exists κ''; inverts Htail; simpl; reflexivity
 |inversion Htail as [|? ? ? Htail']; subst;
   [(* tail base case: κ = κ' *) exists κ''; unfold replacetail_kont; split_refl kont_eq_dec (φ :: κ_)
   |destruct (kont_eq_dec (φ :: κ_) κ') as [Heq | Hneq];
@@ -1187,79 +1078,10 @@ Proof.
     |rewrite no_longer_tail_replacement with (κmore := [φ' ; φ]); [reflexivity | simpl; omega]].
 Qed.
 
-(*
-Require Import Setoid.
-
-
-Lemma no_longer_tail_replacement : forall κ κ' κ'' κmore,
-                                     length κmore > 0 ->
-                                     ~ Tail_replacement κ (κmore ++ κ) κ' κ''.
-Proof.
-  induction κ as [|φ κ_].
-  intros; intro bad; inversion bad; rewrite app_nil_r in H2; contradict H; subst; simpl; omega.
-  intros; intro bad; inversion bad; subst.
-  apply no_circular_app in H2; [contradiction|assumption].
-  assert (~ Tail_replacement κ_ ((κmore ++ [φ]) ++ κ_) κ' κ''').
-  apply IHκ_ with (κmore := κmore ++ [φ]).
-  rewrite app_length; omega.
-  rewrite app_assoc_reverse in H0; simpl in H0; contradiction.
-Qed.
-
-Lemma replace_is_replacement : forall κ κ' κ'' κ''',
-                       (Tail_replacement κ κ' κ'' κ''' <-> replacetail_kont κ κ' κ'' = Some κ''').
-Proof.
-  induction κ as [|φ κ_ IH];
-  [(* base case *)
-  intros; inversion H; subst; split; intro H'; inversion H'; subst; simpl; constructor; auto
-  |
-  intros; inversion H; subst; split; intro H';
-  [(* inversion case 1, first split *)
-  inversion H' as [| foo bar baz qux boo baa]; subst; unfold replacetail_kont; split_refl kont_eq_dec (φ :: κ_);
-    inversion baa; [match goal with [B : ?k = ?f :: ?k |- _] => apply no_circular_cons in B; contradiction end
-                 |subst;apply no_longer_tail_replacement with (κmore := [φ]) in baa; [contradiction|simpl;omega]]
-  (* second split *)
-  |unfold replacetail_kont in H'; split_refl kont_eq_dec (φ :: κ_);
-  injection H'; intros; subst; constructor; auto
-  (* inversion case 2, first split *)
-  |inversion H'; subst;
-   [unfold replacetail_kont; split_refl kont_eq_dec (φ0 :: κ'0)
-   |rewrite IH in H6;
-   apply kont_tail_cons in H; auto]
-  |]].
-
-  unfold replacetail_kont; fold replacetail_kont; rewrite H6;
-  destruct (kont_eq_dec (φ :: κ_) (φ0 :: κ'0)) as [Heq | Hneq];
-    [inversion H0; subst;
-     [apply no_circular_app with (l := [φ0]) in Heq; [contradiction|simpl;omega]
-     |injection Heq; intros; subst;
-      assert (bad : replacetail_kont (φ1 :: κ') (φ0 :: φ1 :: κ') κ'' = None) by
-          (apply no_longer_tail_replacement2 with (κmore := [φ0]); simpl; auto);
-      rewrite bad in H6; discriminate]
-    |auto].
-
-  unfold replacetail_kont in H'; fold replacetail_kont in H'.
-  destruct (kont_eq_dec (φ :: κ_) (φ0 :: κ'0)) as [Heq | Hneq];
-    [injection H'; injection Heq; intros; subst; constructor
-    |].
-  
-  assert (R : exists κ''_, (replacetail_kont κ_ (φ0 :: κ'0) κ'') = Some κ''_).
-  destruct (replacetail_kont κ_ (φ0 :: κ'0) κ'') as [κ''_|];
-    [injection H';intros;subst; exists κ''_; auto
-    |discriminate].
-  destruct R as [κ''_ repeq].
-  assert (R' : φ :: κ''_ = κ''').
-  destruct (replacetail_kont κ_ (φ0 :: κ'0) κ'') as [κ''__|];
-    [injection H'; injection repeq; intros; subst; auto
-    |discriminate].
-  rewrite <- R'.
-  apply push_replacement.
-  rewrite <- IH in repeq; [| apply kont_tail_cons in H]; auto.
-Qed.
-*)  
-
 Inductive ctx_of : TrunKont -> Context -> Prop :=
   | push_ctx : `{ctx_of tκ ctx -> ctx_of (kpush φ tκ) ctx}
   | rt_ctx : `{ctx_of (rt ctx) ctx}.
+Hint Constructors ctx_of.
 
 Fixpoint get_ctx (tκ : TrunKont) : option Context :=
   match tκ with
@@ -1268,9 +1090,9 @@ Fixpoint get_ctx (tκ : TrunKont) : option Context :=
     | rt ctx => Some ctx
   end.
 Theorem reflect_ctx : forall tκ ctx, ctx_of tκ ctx <-> get_ctx tκ = Some ctx.
-Proof. induction tκ; split; intro H; simpl; solve [inversion H; constructor; auto
-                                                  |constructor; rewrite IHtκ; auto
-                                                  |inversion H; subst; simpl; rewrite <- IHtκ; auto].
+Proof. induction tκ; intuition solve [inversion H; auto
+                                     |constructor; rewrite IHtκ; auto
+                                     |inverts H; simpl; rewrite <- IHtκ; auto].
 Qed.
 
 Definition ctx_in_dom (Ξ : KTable) (tκ : TrunKont) :=
@@ -1415,6 +1237,7 @@ Proof.
     |(* do ap : ε *)
      ε s0'eq p0' κ0' t0' pp κt_ ts seq Ht_ H_ πeq (shell p κ_ t) (ap x e ρ v σ) (ev e ρ' σ') π' σ].
 Qed.
+End StackIrrelevance.
 
 Definition Context_inv :=
   (fun p tκ M Ξ ctx =>
@@ -1444,7 +1267,7 @@ Definition ContextLE (ctx ctx' : Context) : Prop :=
   end.
 Definition KTableOrd (Ξ : KTable) := forall ctx tκ (Hin : in_ctxs Ξ ctx tκ) ctx' (Hctx : ctx_of tκ ctx'), ContextLE ctx' ctx /\ InDom Ξ ctx'.
 Definition MTableOrd (M : Memo) := forall e ρ σ t vm σm tm (Hin : in_memos M (context e ρ σ t) (res vm σm tm)), MappingLE σ σm.
-Inductive StateOrd : CESKMΞ -> Prop :=
+Inductive StateOrd : WCESKMΞ -> Memo -> KTable -> Prop :=
   stateord_intro : forall p tκ t M Ξ
                           (Mord : MTableOrd M)
                           (Kord : KTableOrd Ξ)
@@ -1456,7 +1279,7 @@ Inductive StateOrd : CESKMΞ -> Prop :=
                                             (context _ _ σ _) => MappingLE σ (store_of p)
                                         end
                                     end),
-                     StateOrd (widemk (wshell p tκ t) M Ξ).
+                     StateOrd (wshell p tκ t) M Ξ.
 
 Lemma InDom_join : forall Ξ ctx tκ, InDom (Ξ_join Ξ ctx tκ) ctx.
 Proof.
@@ -1482,7 +1305,14 @@ rewrite (InDom_In context_eq_dec) in H;
 inversion H as [b ?]; apply In_join with (b := b); solve [auto | exact context_eq_dec].
 Qed.
 
-Lemma ord_invariant : forall s s' (Hstep : red_ceskmk s s') (Hinv : StateOrd s), StateOrd s'.
+(* This ordering invariant I believe is important to make sure that unrolled continuations
+   cannot refer to a table extension "deep" in the unrolling. The contexts a continuation is
+   unrolled through are partially ordered, so once the contexts differ, no "later" unrolling can
+   use the trunkonts mapped at that context.
+XXX: This still leaves the tricky case of [ctx ↦ ...rt ctx...].*)
+Lemma ord_invariant : forall s M Ξ s' M' Ξ'
+                             (Hstep : red_ceskmk (widemk s M Ξ) (widemk s' M' Ξ'))
+                             (Hinv : StateOrd s M Ξ), StateOrd s' M' Ξ'.
 Proof.
 intros;
   inversion Hinv;
@@ -1534,538 +1364,122 @@ intros ctx' tκ' Hin ctx'' Hctx;
                [apply maple_trans with (l' := σ); [|apply σ_join_ordering]; auto
                |apply InDom_join2]
               |destruct (Kord _ _ S1 ctx'' Hctx); split; [|apply InDom_join2]]; auto].
-
+(* memoized ap context ordering *)
 subst p; simpl;
 destruct (get_ctx tκ) as [[e'' ρ'' σ'' t'']|]; destruct ctxord; split; [apply InDom_join2|];auto;
 apply maple_trans with (l' := σ'); [apply maple_trans with (l' := σ);[|apply σ_join_ordering]|apply (Mord _ _ _ _ _ _ _ Hinmemos)];auto.
 
-injection Hpeq; intros; subst M t tκ p Ξ; simpl in ctxord; destruct ctxord;
-intros ce cρ cσ ct cvm cσm ctm Hinmemos.
+(* memoizing memo table ordering *)
+unfold MTableOrd; (* injection Hpeq; *) intros; subst; simpl in ctxord; destruct ctxord.
+(* intros ce cρ cσ ct cvm cσm ctm Hinmemos. *)
 destruct (in_list_join_set_split context_eq_dec result_eq_dec)
-                       with (l := Ms) (l' := Ms) (a := ctx) (a' := (context ce cρ cσ ct)) (c := (res v σ t's)) (c' := (res cvm cσm ctm))
+                       with (l := M) (l' := M) (a := ctx) (a' := (context e ρ σ0 t0)) (c := (res v σ (tick (co v σ)))) (c' := (res vm σm tm))
                        as [[mum ble]|S1]; auto.
 destruct ctx as [? ρblah σblah ?];
-  injection mum; intros; subst ce cρ cσ ct;
-  injection ble; intros; subst cvm cσm ctm; auto.
+  injection mum; intros; subst e ρ σ0 t0;
+  injection ble; intros; subst vm σm tm; auto.
 pose (grumble := Mord _ _ _ _ _ _ _ S1); auto.
 
-injection Hpeq; intros; subst M t tκ p Ξ; simpl in ctxord; destruct ctxord; destruct ctx as [? ρblah σblah ?];
+subst; simpl in ctxord; destruct ctxord; destruct ctx as [? ρblah σblah ?];
 case_eq (get_ctx tκs); [intros [e_ ρ_ σ_ t_] Hctxeq; rewrite <- reflect_ctx in Hctxeq; simpl;
                         pose (mumble := Kord _ _ Hin_ctxs _ Hctxeq);
                         simpl in mumble; destruct mumble; split; [|apply maple_trans with (l' := σblah)]|];auto.
 Qed.
 
-Remark ord_invariant0 : forall e, StateOrd (inject_ceskmk e).
+Remark ord_invariant0 : forall e, StateOrd (inject_wceskmk e) nil nil.
 intro e; apply stateord_intro;
 [intros ? ? ? ? ? ? ? H|intros ? ? H|simpl; trivial]; inversion H as [? [bad ?]]; inversion bad.
 Qed.
 
-Lemma join_unroll_ordered : forall Ξ ctx ctx' tκ tκ' κ,
-                              KTableOrd Ξ ->
-                              in_ctxs_tail Ξ ctx' tκ' ->
-                              (* If ctx is the ctx_of tκ', but tκ <> tκ', we have a bit of a problem.
-                                 Unwinding tκ' past its rt can lead to using tκ in κ, but this may not
-                                 have been possible prior to the join..
-                               *)
-                              StackUnroll (Ξ_join Ξ ctx tκ) κ tκ' ->
-                              (ctx' <> ctx
-                               \/
-                               (match get_ctx tκ' with
-                                    None => True
-                                  | Some ctx'' => ((ctx'' <> ctx) \/ ctx'' <> ctx')
-                                end))                              
-                                ->
-                                StackUnroll Ξ κ tκ'.
-Proof.
-  intros Ξ ctx ctx' tκ tκ' κ Kord Hctx Hunroll; induction Hunroll; intro Hget.
-  
-  constructor.
-  
-  constructor; apply IHHunroll;
-  [destruct Hctx as [tκ0_ [Htailin Htail]];
-    exists tκ0_; split; [assumption|inversion Htail; subst; [do 2 constructor|apply trunkont_tail_kpush with (φ := φ); auto]]
-  |inversion Hget as [neq1 | hmatch];[left; exact neq1|right; simpl in hmatch; assumption]].
-  
-  destruct (in_list_join_set_split context_eq_dec trunkont_eq_dec Ξ Ξ ctx tκ H) as [[ctxeq tκeq]|Hinrest].  
-
-  subst; inversion Hget as [neq1 | hmatch].
-  destruct Hctx as [mum [ble grmbl]].
-  inversion grmbl; subst.
-  apply IHHunroll.
-  pose (what := Kord _ _ ble ctx0 rt_ctx).
-
-  unfold KTableOrd in Kord.
-
-
-  induction tκ' as [| | ctx'']; intros κ Kord Hctx Hunroll Hget.
-  inversion Hunroll; subst; constructor.
-  inversion Hunroll; subst; constructor; apply IHtκ'; auto.
-  simpl in Hget; destruct (get_ctx tκ') as [ctx_|]; [repeat split|trivial];
-  destruct Hget as [Hctx [Hindom [Hneq|[Heq Hneq]]]]; auto.
-  subst; right; split; auto.
-  inversion Hunroll as [| |? ? ? Hunroll' Hinctx]; subst; simpl in Hget.
-
-  subst; apply unroll_rt with (tκ := tκ0).
-
-Inductive Inv : CESKMΞ -> Prop :=
-  inv : forall p tκ t M Ξ,
+Inductive WInv : WCESKMΞ -> Memo -> KTable -> Prop :=
+  winv : forall p tκ t M Ξ,
           Dom_in_Dom M Ξ ->
           ctx_in_dom Ξ tκ ->
           (forall ctx', (InDom Ξ ctx') -> Context_inv p tκ M Ξ ctx')
            ->
-          Inv (widemk (wshell p tκ t) M Ξ).
+          WInv (wshell p tκ t) M Ξ.
+  
+Inductive Inv : CESKMΞ -> Prop :=
+  inv : forall s M Ξ, WInv s M Ξ -> Inv (widemk s M Ξ).
 
-Lemma inv_invariant : forall s s', Inv s -> StateOrd s -> red_ceskmk s s' -> Inv s'.
+Inductive WideInv : System -> Prop :=
+  wideinv : forall Seen F M Ξ
+                (SeenInv : forall s, set_In s Seen -> WInv s M Ξ /\ StateOrd s M Ξ)
+                (FrontierInv : forall s, set_In s F -> WInv s M Ξ /\ StateOrd s M Ξ),
+           WideInv (system Seen F M Ξ).
+
+Lemma inv_invariant : forall s M Ξ s' M' Ξ', WInv s M Ξ -> StateOrd s M Ξ -> red_ceskmk (widemk s M Ξ) (widemk s' M' Ξ') -> WInv s' M' Ξ'.
 Proof.
-  intros s s' Hinv Hord Hstep.
-  inversion Hord as [? ? ? ? ? Mord Kord ctxord];
-  inversion Hinv as [? ? ? ? ? Hdom tκctx Φ seq]; subst; injection seq; intros; subst; clear seq.
-  Ltac doinvert Un κ tκ φ H ctx Hin :=
-    inversion Un as [|κ tκ φ H|ctx tκ κ H Hin];
-    try (set (ctx := (context (var 0) (@nil (Name * Addr)) (@nil (Addr * AbsVal))));
-         set (Hin := 0)).
-  Ltac noinvert Un κ tκ φ H ctx Hin := set (κ := (@nil Frame));
-                                       set (tκ := mt);
-                                       set (φ := (ar (var 0) (@nil (Name * Addr))));
-                                       set (H := 0);
-                                       set (ctx := (context (var 0) (@nil (Name * Addr)) (@nil (Addr * AbsVal))));
-                                       set (Hin := 0).
-  Ltac part1 ctx tκctx := apply inv; try solve [apply unroll_push; auto
-                           |repeat constructor; auto
-                           |auto
-                           |apply Dom_join_left; firstorder
-                           |apply Dom_join_right; firstorder
-                           |intros blah blorg; apply tκctx; inversion blorg; subst; auto
-                           |inversion Hctx; subst; try solve [discriminate
-                                                              |constructor; auto
-                                                             |auto]].
-  set (idκ := fun κ : Kont => κ).
-  Ltac part2 p Φ M Ξ inpoint fnκ trypop :=
-    let κ' := fresh "κ'" in
-    let κ'' := fresh "κ''" in
-    let φ := fresh "φ" in
-    intros [ce cρ cσ ct] Hindom tκ' Hinctx;
-    constructor;
-    [(* reach *)
-      destruct (Φ (context ce cρ cσ ct) Hindom tκ') as [Hreach Hmemo]; auto;
-     subst p; auto;
-     intros κ' unroll'; pose (Hreach' := Hreach κ' unroll'); destruct Hreach' as [κ [eunroll [t' [t'' [π HT]]]]];
-     ((trypop;
-       match goal with
-           [H : StackUnroll Ξ ?κ (kpush (ar ?e ?ρ) ?tκ) |- _] =>
-           pose (φ := (ar e ρ)); inversion H as [|κ''|]
-       | [H : StackUnroll Ξ ?κ (kpush (fn ?v) ?tκ) |- _] =>
-         pose (φ := (fn v)); inversion H as [|κ''|]
-       end;
-       exists (fnκ κ κ'' φ))
-        || exists (fnκ κ));
-      split; [|exists t', (tick inpoint)];
-     [|exists (shell inpoint κ t'' :: π)]; subst; repeat constructor; auto
-    |(* memo *)
-    let v := fresh "v" in
-    intros v σ'' t' Hmemo;
-      assert (HindomM : InDom M (context ce cρ cσ ct)) by
-        (destruct Hmemo as [ress [Hmapress Hinress]]; rewrite InDom_is_mapped; [exists ress|exact context_eq_dec]; auto);
-      assert (HindomΞ : InDom Ξ (context ce cρ cσ ct)) by (apply Dom_InDom with (l := M); [exact context_eq_dec| | ]; auto);
-      destruct (Φ (context ce cρ cσ ct) HindomΞ tκ'); auto]. 
+Admitted.
 
-  inversion Hstep as [x ρ σ a tκs ts Ms Ξs ps Hmap Hpeq Hs'eq |
-                      e0 e1 ρ σ tκs ts Ms Ξs ps Hpeq |
-                      x e ρ σ tκs ts Ms Ξs ps Hpeq Hs'eq |
-                      v σ e ρ tκs ts Ms Ξs ps Hpeq Hs'eq |
-                      v σ x e ρ fnv tκs ts Ms Ξs ps Hin_force Hpeq Hs'eq |
-                      x e ρ v σ tκs ts Ms Ξs ps a ρ' σ' ts' ctx Hunmapped Hpeq Hs'eq |
-                      x e ρ v σ tκs ts Ms Ξs vm σm tm ps a ρ' σ' ctx Hinmemos Hpeq Hs'eq |
-                      v σ ctx tκs Ms Ξs t's M's Hin_ctxs Hpeq Hs'eq]; subst;
-  [(* var: ε *)
-    constructor; auto; part2 p Φ M Ξ (ev (var x) ρ σ) idκ fail
-   |(* app: push *)
-   constructor; auto;
-   [(* ctx_in_dom *)
-     intros ctx Hctx; destruct (tκctx ctx); inversion Hctx; auto
-    |part2 p Φ M Ξ (ev (app e0 e1) ρ σ) (fun (κ : Kont) => (ar e1 ρ :: κ)) fail]
-   |(* lam: ε *)
-    constructor; auto; part2 p Φ M Ξ (ev (lam x e) ρ σ) idκ fail
-   |(* ar : exchange *)
-    constructor; auto;
-    [intros ctx Hctx; destruct (tκctx ctx) as [X]; inversion Hctx; subst; [constructor|exists X]; auto
-    |part2 p Φ M Ξ (co v σ) (fun (κ κ' : Kont) (φ : Frame) => (fn v :: κ')) idtac]
-   |(* fn -> ap : pop *)
-   constructor; auto;
-    [intros ctx Hctx; destruct (tκctx ctx) as [X]; inversion Hctx; subst;
-     solve [constructor; auto | exists X; auto]
-    |part2 p Φ M Ξ (co v σ) (fun (κ κ' : Kont) (φ : Frame) => κ') idtac]
-   |(* do ap : ε *)
-   constructor; auto
-   |(* ap memo : ? *)
-   |(* ret: pop *)].
+Lemma step_all_invariant : forall s M Ξ, WInv s M Ξ -> StateOrd s M Ξ -> Forall Inv (step_all (widemk s M Ξ)).
+Proof.
+intros ? ? ? Hwinv Hoinv; rewrite Forall_forall; intros [? ? ?]; rewrite <- finite_steps; intros;
+exact (inv (inv_invariant Hwinv Hoinv H)).
+Qed.
 
-  apply Dom_join_right; firstorder.
-  intros ctx' Hctx'; inversion Hctx'; subst; try solve [discriminate
-                                                              |constructor; auto
-                                                             |auto].
+Lemma step_all_ord_invariant : forall s M Ξ, StateOrd s M Ξ -> Forall (fun ws => match ws with widemk s' M' Ξ' => StateOrd s' M' Ξ' end) (step_all (widemk s M Ξ)).
+Proof.
+intros ? ? ? Hoinv; rewrite Forall_forall; intros [? ? ?]; rewrite <- finite_steps; intros;
+exact (ord_invariant H Hoinv).
+Qed.
 
-  destruct (in_list_join context_eq_dec
-                         κs_join
-                         κ_singleton
-                         κs_join_extensive
-                         κ_singleton_extensive
-                         Ξ Ξ
-                         (context e ρ' σ' ts')
-                         tκ
-                         (fun (ab : Context * TrunKonts) (H : In ab Ξ) => H)) as [omg [? ?]];
-    exists omg; apply MapsTo_In; auto.
-    let κ' := fresh "κ'" in
-    let κ'' := fresh "κ''" in
-    let φ := fresh "φ" in
-    intros [ce cρ cσ ct] Hindom tκ' Hinctx;
-    constructor.
-    (* reach *)
-    intros κ' unroll';
-    destruct (in_list_join_set_split context_eq_dec trunkont_eq_dec Ξ Ξ ctx tκ Hinctx) as [[ctxeq tκeq]|Hinrest];
-    [subst; injection ctxeq; intros; subst ce cρ cσ ct;
-     exists κ'; split;[apply unroll_rt with (tκ := tκ'); auto |exists ts',ts',nil; constructor]
-    |assert (Hneed : InDom Ξ (context ce cρ cσ ct)) by
-        (destruct Hinrest as [tκs [Hmap ?]]; rewrite InDom_is_mapped; [exists tκs|exact context_eq_dec]; auto);
-      destruct (Φ (context ce cρ cσ ct) Hneed tκ') as [Hreach Hmemo]; auto].                              
-    .
-(* Stuck *)
-    destruct Hreach as 
-    [(* reach *)
-      
-      
-     subst p; auto;
-     intros κ' unroll'; pose (Hreach' := Hreach κ' unroll'); destruct Hreach' as [κ [t' [t'' [eunroll [π HT]]]]];
-     exists (rt ctx);
-     exists t', (tick (ap x e ρ v σ)); split;
-     [|exists (shell (ap x e ρ v σ) κ t'' :: π)]; subst; repeat constructor; auto
-    |(* memo *)
-    let v := fresh "v" in
-    intros v σ'' t' Hmemo;
-      assert (HindomM : InDom M (context ce cρ cσ ct)) by
-        (destruct Hmemo as [ress [Hmapress Hinress]]; rewrite InDom_is_mapped; [exists ress|exact context_eq_dec]; auto);
-      assert (HindomΞ : InDom Ξ (context ce cρ cσ ct)) by (apply Dom_InDom with (l := M); [exact context_eq_dec| | ]; auto);
-      destruct (Φ (context ce cρ cσ ct) HindomΞ tκ'); auto]. 
+Definition TableContains (M : Memo) (Ξ: KTable) (ss : set CESKMΞ) :=
+  Forall (fun s => match s with widemk ws M' Ξ' => MappingLE M' M /\ MappingLE Ξ' Ξ end) ss.
 
-  part2 p Φ M Ξ (ap x e ρ v σ) (fun (κ κ' : Kont) (φ : Frame) => (rt ctx)) fail.
-                         (*                          (l := Ξ) (l' := Ξ)
+Lemma smush_invariant : forall Seen ss M Ξ nexts
+                               (SeenInv : Forall (fun s => WInv s M Ξ) Seen)
+                               (MΞinv : TableContains M Ξ ss)
+                               (ssInv : Forall Inv ss)
+                               (nextsInv : Forall (fun s => WInv s M Ξ) nexts),
+                          match smusher Seen ss nexts M Ξ with
+                              wide_step ss M' Ξ' => Forall (fun s => WInv s M' Ξ') ss
+                          end.
+Proof.
+  induction ss as [|[s' M' Ξ'] ss' IH]; intros.
+  (* base *)
+  simpl; rewrite Forall_forall; intros s H; rewrite filter_In in H; destruct H as [Hin feq];
+  rewrite Forall_forall in nextsInv; apply nextsInv; auto.
+  (* induction step *)
+  simpl.
+apply IH.
+Focus 2.
+unfold TableContains; rewrite Forall_forall;
+unfold TableContains in MΞinv; rewrite Forall_forall in MΞinv;
+intros mum ble; assert (blahneed : In mum (widemk s' M' Ξ' :: ss')) by (right; exact ble); pose (blah := (MΞinv mum blahneed));
+destruct mum; intuition ((apply maple_trans with (l' := M) || apply maple_trans with (l' := Ξ)); solve [apply map_join_ordering2; auto | auto]).
+Focus 2.
+rewrite Forall_forall; rewrite Forall_forall in ssInv; intros mum ble; apply ssInv; right; auto;
+pose (useIH := IH (Ms_join M' M) (Ξs_join Ξ' Ξ) (set_add wceskmξ_eq_dec s' nexts)).
+Abort.
 
-(a := (context e ρ' σ' ts'))
-                         (c := tκ) *)). forall l l' a c,
-    (forall ab, In ab l -> In ab l') ->
-  in_list_list (list_join eq_dec combine base l' a c l) a c.
-
-
-  unfold
-  apply in_list_join.
-  apply Dom_in_D
-    constructor; auto; part2 p Φ M Ξ (ap x e ρ v σ) idκ fail
-  .
-    
-  part2 p Φ M Ξ (ev (app e0 e1) ρ σ) (fun (κ κ' : Kont) (φ : Frame) => (ar e1 ρ :: κ')) idtac.
-
-  constructor; auto.
-  intros ctx Hctx; destruct (tκctx ctx) as [X]; inversion Hctx; subst; [constructor|exists X];auto.
-  intros [ce cρ cσ ct] Hindom tκ' Hinctx;
-    constructor;
-    [(* reach *)
-      destruct (Φ (context ce cρ cσ ct) blarg tκ') as [Hreach Hmemo]; auto;
-     subst p; auto;
-     intros κ' unroll'; pose (Hreach' := Hreach κ' unroll'); destruct Hreach' as [κ [t' [t'' [eunroll [π HT]]]]]
-     |].
-     ;
-     exists (fnκ κ), t', (tick inpoint); split;
-     [|exists (shell inpoint κ t'' :: π)]; repeat constructor; auto
-    |(* memo *)
-    let v := fresh "v" in
-    intros v σ'' t' Hmemo;
-      assert (HindomM : InDom M (context ce cρ cσ ct)) by
-        (destruct Hmemo as [ress [Hmapress Hinress]]; rewrite InDom_is_mapped; [exists ress|exact context_eq_dec]; auto);
-      assert (HindomΞ : InDom Ξ (context ce cρ cσ ct)) by (apply Dom_InDom with (l := M); [exact context_eq_dec| | ]; auto);
-      destruct (Φ (context ce cρ cσ ct) HindomΞ tκ'); auto]. 
-
-  part2 p Φ M Ξ (co v σ) (fun κ => (fn v :: κ)).
-
-  Ltac solve_inner point t reach :=
-    let tκ' := fresh "tκ'" in
-    let cκ := fresh "cκ" in
-    let cunroll := fresh "cunroll" in
-    let creach := fresh "creach" in
-    let cmemo := fresh "cmemo" in
-    let t'_ := fresh "t'_" in
-    let π := fresh "π" in
-    let chκ := fresh "chκ" in
-    let cH := fresh "cH" in
-    split; [assumption
-           |split;[intros chκ cH; destruct (reach chκ) as [t'_ [π ?]];
-                   try solve [auto | constructor; auto];
-                   exists t'_;
-                   exists (Cons (shell point chκ t) π);
-                   constructor; [assumption
-                                |compute; rewrite <- comparable_ticks with (κ := chκ);
-                                 solve [repeat constructor; auto | auto]]
-                  |]];
-    repeat constructor; auto.
-  (* Var lookup *)
-  subst; part1 (context ce cρ cσ) tκctx. 
-  intro tκ'; destruct (Hctx tκ') as [cκ [cunroll [creach cmemo]]];
-  exists cκ; solve_inner (ev (var x) ρ σ) t creach.
-  intros [cce ccρ ccσ] ccH; pose (Φinst := Φ (context cce ccρ ccσ) ccH); simpl in Φinst.
-  intro tκ'; destruct (Φinst tκ') as [κ' [un' [reach' memo']]];
-  exists κ'; solve_inner (ev (var x) ρ σ) t reach'.
-  (* function eval *)
-  subst; part1 (context ce cρ cσ) tκctx.
-  intro tκ'; destruct (Hctx (kpush (ar e1 ρ) tκ')) as [cκ [cunroll [creach cmemo]]].
-  exists cκ_;
-    split; [assumption
-           |split;[intros chκ cH
-                                                            |]].
-  destruct (creach ((ar e1 ρ)::cκ_)) as [t'_ [π ?]]
-    inversion cH; subst; auto.
-                   try solve [auto | constructor; auto];
-
-
- solve_inner (ev (app e0 e1) ρ σ) t creach.
-  
-  destruct ctx
-  inversion Hctx; subst; try solve [discriminate
-                                                              |constructor; auto
-                                                             |auto].
- part2 Φ mumble t idκ; repeat split; auto.
-    let κ_ := fresh "κ_" in
-    let Hunroll_ := fresh "Hunroll_" in    
-    repeat split; auto;
-    intros κ_ Hunroll_;
-    inversion Hunroll_ as [|κ__ ? ? Hu__|]; subst;
-    destruct (mumble κ__) as [t'_ [π Φreach_path]]; auto;
-    exists t'_;
-        exists (Cons (shell (ev (app e0 e1) ρ σ) κ__ t) π);
-        constructor; [assumption|
-                      compute;
-                        rewrite <- (comparable_ticks _ _ _ (κ := κ__));
-                        solve [constructor; auto
-                              |auto]].
-  (* lam *)
-  subst; part1; part2 Φ mumble t idκ; repeat split; auto.
-    let κ_ := fresh "κ_" in
-    let Hunroll_ := fresh "Hunroll_" in    
-    repeat split; auto;
-    intros κ_ Hunroll_;
-    destruct (mumble κ_) as [t'_ [π Φreach_path]]; auto;
-    exists t'_;
-        exists (Cons (shell (ev (lam x e) ρ σ) κ_ t) π);
-        constructor; [assumption|
-                      compute;
-                        rewrite <- (comparable_ticks _ _ _ (κ := κ_));
-                        solve [constructor; auto
-                              |auto]].  
-  (* evaluated fn, now arg eval *)
-    subst; part1; part2 Φ mumble t idκ; repeat split; auto;
-    let κ_ := fresh "κ_" in
-    let Hunroll_ := fresh "Hunroll_" in    
-    repeat split; auto;
-    intros κ_ Hunroll_;
-    inversion Hunroll_ as [|κ__|]; subst;
-    destruct (mumble ((ar e ρ)::κ__)) as [t'_ [π Φreach_path]];
-      [constructor|];auto;
-    exists t'_;
-        exists (Cons (shell (co v σ) ((ar e ρ)::κ__) t) π);
-        constructor; [assumption
-                     |compute; rewrite <- (comparable_ticks _ _ _ (κ := ((ar e ρ)::κ__)));
-                      solve [constructor; auto | auto]].
-  (* fn -> ap *)
-    subst; part1; part2 Φ mumble t idκ; repeat split; auto.
-    let κ_ := fresh "κ_" in
-    let Hunroll_ := fresh "Hunroll_" in    
-    repeat split; auto;
-    intros κ_ Hunroll_;
-    destruct (mumble ((fn fnv)::κ_)) as [t'_ [π Φreach_path]];
-    [constructor|]; auto;
-    exists t'_;
-        exists (Cons (shell (co v σ) ((fn fnv)::κ_) t) π);
-        constructor; [assumption|
-                      compute;
-                        rewrite <- (comparable_ticks _ _ _ (κ := ((fn fnv)::κ_)));
-                        solve [constructor; auto
-                              |auto]].
-  (* do unmemoized ap *)
-    part1.
-    constructor.
-    destruct in_list_join with (eq_dec := context_eq_dec) (combine := κs_join) (base := κ_singleton)
-                                                          (l := Ξ) (l' := Ξ) (a := ctx) (c := tκ)
-                                                          as [κs [? ?]];
-      [intros; apply set_add_intro2
-       |intros; simpl
-       |
-      |exists κs;apply MapsTo_In]; auto.    
-    let e' := fresh "e'" in
-    let ρ'' := fresh "ρ''" in
-    let σ'' := fresh "σ''" in
-    let tκ' := fresh "tκ'" in
-    let κ' := fresh "κ'" in
-    let Htκ' := fresh "Htκ'" in
-    let Hunroll:= fresh "Hunroll" in
-    intros e' ρ'' σ'' tκ' Htκ'.
-    destruct (in_list_join_set_split context_eq_dec trunkont_eq_dec)
-    with (l := Ξ) (l' := Ξ) (a := ctx) (a' := (context e' ρ'' σ'')) (c := tκ) (c' := tκ')
-                  as [[? ?]|ble];
-      [unfold in_ctxs in Htκ'; auto
-      |(* considered context is the one we extended Ξ with *)
-      subst ctx;
-        match goal with [H : (context ?uu ?vv ?hh) = (context ?ww ?xx ?yy) |- _] =>
-                        injection H; intros aaa bbb ccc; subst ww xx yy end
-      |].
-    inversion Hctx as [HH|? ? HH|? HH].
-    (* mt case *)
-    assert (R : tκ' = mt) by congruence; rewrite R.
-    exists nil; repeat constructor; auto.
-    subst p.
-    pose (mar := Φ e ρ' σ' tκ').
-    
-    
-match goal with [H' : mt = t
-    destruct (Φ e ρ' σ' tκ0) as [stuff boo].
-    injection H3; intros aaa bbb ccc; subst e' ρ'' σ''.
-    
-    [apply in_list_join2
-      |
-      |].
-
-    
-
-    Check in_list_join_split.
-    destruct (in_list_join_split context_eq_dec κs_join κ_singleton) with
-      (l := Ξ)
-      (l' := Ξ)
-      (a := ctx)
-      (a' := (context e' ρ'' σ''))
-      (c := tκ)
-      (c' := tκ') as [S0|[S1|S2]]; auto.
-    destruct (Φ e' ρ'' σ'' tκ' S0) as [κseen [seenunroll [seenreach seenmemo]]].
-    exists κseen; repeat split;
-    [apply unroll_with_extension
-    |intros κreach reachunroll
-    |]; auto.
-
-
-; specialize seenreach with κreach
- [intros;  | ]; auto.
-.: forall l l' a a' c c'
-                             (Hcontain : (forall ab, In ab l -> In ab l')),
-    
-    destruct Φrinst as [κ' [Hunroll [Φreach Φmemo]]].
-    exists (κfn1 κ').
-
-
- part2 Φ mumble t idκ; repeat split; auto.
-  Focus 3.
-  (* return and memoize *)
-  inversion Htail as [| | ? ? ? Hunroll Hctxin]; subst;
-  [discriminate
-  |discriminate
-  |match goal with [H : rt ?ctx0 = rt ctx |- _] => injection H; intros; subst end].
-  destruct ctx as [e_ ρ_ σ_];
-    destruct (Φ e_ ρ_ σ_ tκ' Hin_ctxs) as [κ' [? [? ?]]].
-
-  apply (inv (κ := κ')); try solve [apply unroll_push; auto
-                                  |constructor; auto
-                                  |auto
-                                  |apply Dom_join_left; firstorder].
-  intros e'' ρ'' σ'' tκ'' Htκ'';
-    pose (Φrinst := (Φ e'' ρ'' σ'' tκ'' Htκ''));
-    destruct Φrinst as [κ'' [Hunroll' [Φreach Φmemo]]];
-    exists κ'';
-    destruct Φreach as [t'_ [π Φreach_path]];
-    repeat split; [auto
-                  |exists t'_|].
-
- solve [auto |
-      (* reach *)
-      exists t'_;
-        exists (Cons (shell (co v σ) (rt (context e_ ρ_ σ_)) t) π);
-        constructor; [assumption|
-                      compute;
-                        rewrite <- (comparable_ticks _ _ _ (κ := κ));
-                        solve [constructor; auto
-                              |auto]]
-            |(* memo *) auto].
-      part2 Φ point κ t.
-
-  subst; common Φ κ' (co v σ) κ t.
-  
-  constructor.
-  subst; common Φ κ (co v σ) (rt ctx) t.
-
-  apply inv with (κ := κ); auto; subst.
-  (* satisfy hyps of inv first *)
-  apply Dom_join_right; auto.
-  apply unroll_rt with (tκ := tκ); [apply unroll_with_extension; auto
-                                   |apply in_list_join; solve [
-                                                            intros; apply set_add_intro1; auto
-                                                          | intros; apply set_add_intro2; auto 
-                                                          | auto]];
-  subst.
-  intros e'' ρ'' σ'' tκ'' κ'' Htκ'' Hunroll'.
-  destruct (in_list_join_split context_eq_dec
-                               κs_join
-                               κ_singleton
-                               κs_join_extensive
-                               Ξ
-                               Ξ
-                               ctx
-                               tκ
-                               (fun a b => b)
-                               (a' := (context e'' ρ'' σ''))
-                               (c' := tκ'')) as [Hctx|[Hctx|Hctx]];
-    auto.
-  (* first case: already there *)
-  pose (Φrinst := (Φ e'' ρ'' σ'' tκ'' κ'' Hctx)).
-    destruct Φrinst as [Φreach Φmemo];
-    destruct Φreach as [t'_ [π Φreach_path]].
-    
-                               Ξ' (* l *)
-                               Ξ' (* l' *)
-                               ctx (* a *)
-                               (context e'' ρ'' σ'') (* a' *)
-                               tκ (* c *)
-                               tκ'' (* c' *).
-  (* unmemoized ap inv needs to split on ctx mapped before or is new *)
-  part2 Φ (ap x e ρ v σ) κ t.
-  inversion Htκ'' as [tκs [Hinp Hinr]].
-  
-
-  pose (Φparinst := (Φ e'' ρ'' σ'' tκ'' κ'' n'')).
-  red in Hinp.
-  pose (Φrinst := ).
-    destruct Φrinst as [Φreach Φmemo];
-    destruct Φreach as [t'_ [π Φreach_path]].
-
-
-  part2 Φ (ap x e ρ v σ) κ t n.
-  (* do memoized ap *)
-  
-  assert (Htail' : StackUnroll Ξ' κ tκ (ctx :: G)).
-  apply unroll_with_extension with (G := G);[assumption|].
-  apply sublist_extension with (l'' := [ ctx ]).
- with (G' := (set_add context_eq_dec ctx G)); try solve [auto | apply subset_refl].
-  apply unroll_rt with (tκ := tκ); try solve [intro bad; inversion bad].
-  unfold in_ctxs.
-  apply in_list_join; auto;
-  intros; apply set_add_intro2; auto.
-  pose (Φrinst := (Φ e ρ' σ' (rt ctx) κ' Htκ' Htail));
-    destruct Φrinst as [Φreach Φmemo];
-    destruct Φreach as [t'_ [π Φreach_path]].
+Lemma wideinv_invariant : forall Seen F M Ξ Seen' F' M' Ξ'
+                                 (Hinv: WideInv (system Seen F M Ξ))
+                                 (Hstep : Wide_CESKMΞ (system Seen F M Ξ) (system Seen' F' M' Ξ')),
+                            WideInv (system Seen' F' M' Ξ').
+Proof.
+intros; inversion Hstep as [ws ? ? ? F_ Seen_ ? ? Hstepeq]; subst; constructor; intros ws' Hin.
+destruct ws as [[e ρ σ | v σ | x e ρ v σ] tκ t]; [|destruct tκ|].
+(* ev case *)
+destruct e as [x | e0 e1 | x e ]; simpl in Hstepeq.
+Abort.
 
 Inductive state_rel : CESK -> System -> Prop :=
-  point_rel : `{StackUnroll Ξ κ κ' nil ->
-                (In (wshell p κ' t) Seen \/ In (wshell p κ' t) F) ->
-                state_rel (shell p κ t) (system Seen F M Ξ)}.
+  point_rel : forall Ξ κ tκ p t Seen F M,
+                StackUnroll Ξ κ tκ ->
+                (In (wshell p tκ t) Seen \/ In (wshell p tκ t) F) ->
+                state_rel (shell p κ t) (system Seen F M Ξ).
 
-Theorem simulation : forall e s, CESK_trace e π -> exists s', state_rel s s' /\ WCESKMΞ_trace e π'.
+Theorem simulation : forall e π (HT: CESK_trace e π), exists π', WCESKMΞ_trace e π' /\ Forall (fun xy => match xy with (x,y) => state_rel x y end) (combine π π').
 Proof.
-  intros e s π.
-
-
+  intros e π HT; induction HT.
+  exists [(inject_wide_ceskmk e)];
+    split; [constructor
+           |rewrite Forall_forall; simpl; intros [cesk sys Hin]; inversion_clear Hin as [Heq|bad]; [injection Heq; intros; subst;apply point_rel with (tκ := mt); constructor; left; auto|destruct bad]].
+  destruct IHHT as [π' [HT' Hrel]].
+  inversion H as [x ρ σ a κ t p Hmap
+                 | | | | |]; subst.
+  simpl in Hrel.
 End NonStandardSemantics.
 End NonStandardData.
 End StandardSemantics.
